src/SingleValue.v
@@ -26,16 +26,20 @@ Section System.
   Section Spec.
 
     Definition specIdx := 0.
-    Definition specChn := 0. (* A single channel is enough. *)
+    Definition specChn1 := 0.
+    Definition specChn2 := 1.
     Definition valueIdx := 0.
 
-    Section PerExt.
-      Variable extIdx: nat.
+    Definition getSpecExtIdx (idx: nat) :=
+      if eq_nat_dec idx specChn1 then extIdx1 else extIdx2.
+    
+    Section PerChn.
+      Variable chnIdx: nat.
 
-      Definition getReqM := buildMsgId extIdx specIdx "SvmGet" Rq specChn.
-      Definition getRespM := buildMsgId extIdx specIdx "SvmGet" Rs specChn.
-      Definition setReqM := buildMsgId extIdx specIdx "SvmSet" Rq specChn.
-      Definition setRespM := buildMsgId extIdx specIdx "SvmSet" Rs specChn.
+      Definition getReqM := buildMsgId (getSpecExtIdx chnIdx) specIdx "SvmGet" Rq chnIdx.
+      Definition getRespM := buildMsgId (getSpecExtIdx chnIdx) specIdx "SvmGet" Rs chnIdx.
+      Definition setReqM := buildMsgId (getSpecExtIdx chnIdx) specIdx "SvmSet" Rq chnIdx.
+      Definition setRespM := buildMsgId (getSpecExtIdx chnIdx) specIdx "SvmSet" Rs chnIdx.
 
       Definition specGetReq: PMsg :=
         {| pmsg_mid := getReqM;
@@ -57,16 +61,16 @@ Section System.
              fun pre v post => exists n, v = VNat n /\ post@[valueIdx] = Some (VNat n)
         |}.
 
-    End PerExt.
+    End PerChn.
 
     Definition specObj: Object :=
       {| obj_idx := specIdx;
          obj_state_init := [valueIdx <- VNat 0];
          obj_trs :=
-           (specGetReq extIdx1)
-             :: (specSetReq extIdx1)
-             :: (specGetReq extIdx2)
-             :: (specSetReq extIdx2) :: nil
+           (specGetReq specChn1)
+             :: (specSetReq specChn1)
+             :: (specGetReq specChn2)
+             :: (specSetReq specChn2) :: nil
       |}.
     
     Definition spec : System := singleton specObj.
@@ -84,7 +88,7 @@ Section System.
     
     Definition theOtherChild (idx: nat) :=
       if eq_nat_dec idx child1Idx then child2Idx else child1Idx.
-    Definition getExtIdx (idx: nat) :=
+    Definition getImplExtIdx (idx: nat) :=
       if eq_nat_dec idx child1Idx then extIdx1 else extIdx2.
 
     (* Definition valueIdx := 0. *)
@@ -97,10 +101,10 @@ Section System.
     Section Child0.
       Variable childIdx: nat.
 
-      Definition ecGetReqM := buildMsgId (getExtIdx childIdx) childIdx "SvmGet" Rq chnImpl.
-      Definition ecGetRespM := buildMsgId (getExtIdx childIdx) childIdx "SvmGet" Rs chnImpl.
-      Definition ecSetReqM := buildMsgId (getExtIdx childIdx) childIdx "SvmSet" Rq chnImpl.
-      Definition ecSetRespM := buildMsgId (getExtIdx childIdx) childIdx "SvmSet" Rs chnImpl.
+      Definition ecGetReqM := buildMsgId (getImplExtIdx childIdx) childIdx "SvmGet" Rq chnImpl.
+      Definition ecGetRespM := buildMsgId (getImplExtIdx childIdx) childIdx "SvmGet" Rs chnImpl.
+      Definition ecSetReqM := buildMsgId (getImplExtIdx childIdx) childIdx "SvmSet" Rq chnImpl.
+      Definition ecSetRespM := buildMsgId (getImplExtIdx childIdx) childIdx "SvmSet" Rs chnImpl.
 
       Definition ecGetReqOk: PMsg :=
         {| pmsg_mid := ecGetReqM;
@@ -209,9 +213,69 @@ Section Sim.
   Qed.
   Hint Resolve svm_simulation_init.
 
+  Definition svmMsgIdF (imid: MsgId): MsgId :=
+    {| mid_rq := mid_rq imid;
+       mid_rs := specIdx;
+       mid_type := mid_type imid;
+       mid_rqrs := mid_rqrs imid;
+       mid_chn := mid_rs imid |}.
+
+  Definition svmMsgF (imsg: Msg): Msg :=
+    {| msg_id := svmMsgIdF (msg_id imsg);
+       msg_value := msg_value imsg |}.
+
+  Lemma svmMsgF_value:
+    forall m, msg_value (svmMsgF m) = msg_value m.
+  Proof. reflexivity. Qed.
+
+  Definition svmMsgsF (imsgs: list Msg): list Msg :=
+    map svmMsgF imsgs.
+
+  Lemma svmMsgsF_value:
+    forall msgs, map msg_value (svmMsgsF msgs) = map msg_value msgs.
+  Proof.
+    induction msgs; simpl; intros; auto.
+    rewrite IHmsgs; reflexivity.
+  Qed.
+
+  Lemma svmMsgsF_validOuts:
+    forall from msgs, ValidOuts from msgs ->
+                      ValidOuts from (svmMsgsF msgs).
+  Proof.
+  Admitted.
+
   Theorem svm_simulation: Simulates SvmR (impl0 extIdx1 extIdx2) (spec extIdx1 extIdx2).
   Proof.
     unfold Simulates; intros.
+
+    apply step_step_det in H0; inv H0.
+
+    - (* silent *) simpl; eauto.
+
+    - (* internal *)
+      admit.
+
+    - (* external *)
+      rewrite toELabel_Some_1 by assumption.
+      exists {| st_oss := st_oss sst1;
+                st_msgs := distributeMsgs (svmMsgsF emsgs) (st_msgs sst1) |}.
+      exists {| lbl_ins := svmMsgsF emsgs; lbl_hdl := None; lbl_outs := nil |}.
+      split; [|split].
+      + apply step_det_step.
+        destruct sst1 as [oss1 oims1]; simpl.
+        eapply SsdExt with (from:= from); eauto.
+        * intro Hx; elim H1; clear H1.
+          Common.dest_in; simpl; tauto.
+        * destruct emsgs; auto.
+          discriminate.
+        * apply svmMsgsF_validOuts; auto.
+        * clear; induction emsgs; simpl; [apply SubList_nil|].
+          admit.
+      + rewrite toELabel_Some_1 by (destruct emsgs; [auto|discriminate]).
+        rewrite svmMsgsF_value; reflexivity.
+      + inv H.
+        econstructor; eauto.
+        inv H6; [eapply VVM1; eauto|eapply VVM2; eauto|eapply VVS; eauto].
   Admitted.
   Hint Resolve svm_simulation.
 
